Strata/DL/Imperative/StmtSemantics.lean
@@ -7,6 +7,7 @@ module
 
 public import Strata.DL.Imperative.CmdSemantics
 public import Strata.DL.Imperative.Stmt
+public import Strata.DL.Imperative.StmtSemanticsSmallStep
 import Strata.Util.Tactics
 
 ---------------------------------------------------------------------
@@ -14,9 +15,6 @@ import Strata.Util.Tactics
 namespace Imperative
 
 public section
-
-/-- Type of a function that extends the semantic evaluator with a new function definition. -/
-@[expose] abbrev ExtendEval (P : PureExpr) := SemanticEval P → SemanticStore P → PureFunc P → SemanticEval P
 
 mutual
 
